in collisions: fix/clean up games, write intermediate games to delete k and inline v (since here's it's randomly sampled instead of fixed... could we even do the full version of instantiate? would only need for the first oracle call?), and apply dupPros to Qed collisions. need to check: doesn't used adam's work on fixed v + is my numbering right?

src/examples/HMAC_DRBG_nonadaptive.v
@@ -57,8 +57,11 @@ Section PRG.
 the key type is now also Bvector eta, since HMAC specifies that the key has the same size as the output (simplified) *)
 Variable eta : nat.
 
-Variable RndK : Comp (Bvector eta).
-Variable RndV : Comp (Bvector eta).
+(* Variable RndK : Comp (Bvector eta). *)
+(* Variable RndV : Comp (Bvector eta). *)
+(* TODO replace them *)
+Definition RndK : Comp (Bvector eta) := {0,1}^eta.
+Definition RndV : Comp (Bvector eta) := {0,1}^eta.
 
 Variable f : Bvector eta -> Blist -> Bvector eta.
 
@@ -81,6 +84,10 @@ Definition Instantiate : Comp KV :=
   k <-$ RndK;
   v <-$ RndV;
   ret (k, v).
+
+Print Comp.
+SearchAbout Comp.
+Locate "<-$". 
 
 (* save the last v and output it as part of the state *)
 Fixpoint Gen_loop (k : Bvector eta) (v : Bvector eta) (n : nat)
@@ -978,7 +985,7 @@ Definition Gi_rb_bad_no_oracle : Comp bool :=
   let firstInput := to_list v in (* fixed *)
   let nextInput := to_list v' in (* extra input to refresh the v *)
   let outputsAsInputs := firstn (blocksPerCall - 1) (map (fun v => to_list v) bits) in (* only the outputs (so v' is not duplicated) -- we need to remove the last output because that isn't used as an input. OR we can leave it in and get a slightly worse bound. *)
-  ret (hasDups _ (firstInput :: nextInput :: outputsAsInputs ++ (keyInput :: nil))).
+  ret (hasDups _ (keyInput :: firstInput :: nextInput :: outputsAsInputs)).
 
 (* remove the v input, cons the fixed v to the beginning, and map all the bvector outputs to blist. corresponds to Adam's PRF_DRBG_f_bad_2 and PRF_DRBG_G3_bad_2. uses Gen_loop_rb.
 can't use GenUpdate_rb because i need the v and k update inputs *)
@@ -1006,12 +1013,12 @@ Definition GenUpdate_rb_no_k (n : nat)
   ret (v', bits, (to_list v'' ++ zeroes)).
 
 Definition Gi_rb_bad_no_k : Comp bool :=
-  [_, v] <-$2 Instantiate;
+  v <-$ RndV;
   [v', bits, keyInput] <-$3 GenUpdate_rb_no_k blocksPerCall;
   let firstInput := to_list v in (* fixed *)
-  let nextInput := to_list v' in (* extra input to refresh the v *)
-  let outputsAsInputs := firstn (blocksPerCall - 1) (map (fun v => to_list v) bits) in (* only the outputs (so v' is not duplicated) -- we need to remove the last output because that isn't used as an input. OR we can leave it in and get a slightly worse bound *)
-  ret (hasDups _ (firstInput :: nextInput :: outputsAsInputs ++ (keyInput :: nil))).
+  let nextInput := to_list v' in (* extra input to the loop -- the refreshed v *)
+  let outputsAsInputs := firstn (blocksPerCall - 1) (map (fun v => to_list v) bits) in 
+  ret (hasDups _ (keyInput :: firstInput :: nextInput :: outputsAsInputs)).
 
 (* ---- *)
 (* *have* to apply the injection to_list : forall eta, Bvector eta -> Blist, since there's one input of a different length, so skip that game *)
@@ -1036,11 +1043,18 @@ Definition Gi_rb_bad_no_k : Comp bool :=
 (*   | nil => default *)
 (*   | x :: *)
 
-(* inline GenUpdate and Gen_loop, change Gen_loop to a map *)
-(* also put keyInput in a less inconvenient place, order doesn't matter TODO *)
-(* TODO delete extraneous comments *)
+(* inline GenUpdate and Gen_loop, change Gen_loop to a map
+remove v'' from the end (it's never used as an input) and generate it separately
+(only (to_list v'' ++ zeroes) is used as an input *)
+
+(*    Definition PRF_DRBG_G3_bad_3 :=
+     ls <-$ compMap _ (fun _ => {0, 1}^eta) (forNats (pred l));
+     ret (hasDups _ (v_init :: (map injD ls))).
+
+^ why is there a (-1) here? *)
+
 Definition Gi_rb_bad_map : Comp bool :=
-  [_, v] <-$2 Instantiate;
+  v <-$ RndV;
   v' <-$ {0,1}^eta;
   bits <-$ compMap _ (fun _ => {0,1}^eta) (forNats (blocksPerCall - 1)); (* ? *)
   v'' <-$ {0,1}^eta;            (* TODO check if this is ok -- should it be -2 above? *)
@@ -1048,25 +1062,36 @@ Definition Gi_rb_bad_map : Comp bool :=
   let firstInput := to_list v in (* fixed *)
   let nextInput := to_list v' in (* extra input to refresh the v *)
   let keyInput := to_list v'' ++ zeroes in
-  let outputsAsInputs := firstn (blocksPerCall - 1) (map (fun v => to_list v) bits) in (* only the outputs (so v' is not duplicated) -- we need to remove the last output because that isn't used as an input. OR we can leave it in and get a slightly worse bound *)
-  (* TODO is this right, here? *)
-  let lastInput := keyInput in  (* won't be a dup of any previous *)
+  let outputsAsInputs := map (fun v => to_list v) bits in
+  (* took the last block off, so don't need firstn anymore *)
   (* keyInput isn't a dup; firstInput is fixed, and inline nextInput into compMap *)
   ret (hasDups _ (keyInput :: firstInput :: nextInput :: outputsAsInputs)).
 
+(* absorb v' into compMap *)
 Definition Gi_rb_bad_map_inline : Comp bool :=
-  [_, v] <-$2 Instantiate;
-  (* absorb v' into compMap *)
-  bits <-$ compMap _ (fun _ => {0,1}^eta) (forNats blocksPerCall); (* ? *)
+  v <-$ RndV;
+  bits <-$ compMap _ (fun _ => {0,1}^eta) (forNats blocksPerCall); 
   v'' <-$ {0,1}^eta;            (* TODO check if this is ok -- should it be -2 above? *)
-  (* not quite right -- blocksPerCall could be 1 -- TODO fix "last elem" everywhere *)
+  (* not quite right -- blocksPerCall could be 1 -- TODO fix "last elem" everywhere? *)
   let firstInput := to_list v in (* fixed *)
   let keyInput := to_list v'' ++ zeroes in
-  let outputsAsInputs := firstn (blocksPerCall - 1) (map (fun v => to_list v) bits) in (* only the outputs (so v' is not duplicated) -- we need to remove the last output because that isn't used as an input. OR we can leave it in and get a slightly worse bound *)
-  (* TODO is this right, here? *)
-  let lastInput := keyInput in  (* won't be a dup of any previous *)
+  let outputsAsInputs := map (fun v => to_list v) bits in
   (* keyInput isn't a dup; firstInput is fixed, and inline nextInput into compMap *)
   ret (hasDups _ (keyInput :: firstInput :: outputsAsInputs)).
+
+(* keyInput cannot collide with any other input, so remove it and the listifying *)
+Definition Gi_rb_bad_map_no_keyinput : Comp bool :=
+  v <-$ RndV;                   (* is {0,1}^eta, but should I leave it fixed?? TODO*)
+  bits <-$ compMap _ (fun _ => {0,1}^eta) (forNats blocksPerCall); 
+  ret (hasDups _ (v :: bits)).
+
+(* v is randomly sampled here... but sometimes it's fixed (as in PRF_DRBG)? TODO *)
+(* seems too simple *)
+Definition Gi_rb_bad_map_inline_v : Comp bool :=
+  bits <-$ compMap (Bvector_EqDec eta) (fun _ => {0,1}^eta) (forNats (S blocksPerCall)); 
+  ret (hasDups (Bvector_EqDec eta) bits).
+
+(* some of these inlinings can probably be done better in a different order or simultaneously *)
 
 (* todo: get it to a point where I can apply Adam's lemma with a different size *)
 (* specifically figure out how much of it i can reuse.
@@ -1122,6 +1147,18 @@ Proof.
   intros.
 Admitted.
 
+Lemma Gi_rb_bad_eq_7 : 
+    Pr [Gi_rb_bad_map_inline] = Pr [Gi_rb_bad_map_no_keyinput].
+Proof.
+  intros.
+Admitted.
+
+Lemma Gi_rb_bad_eq_8 : 
+    Pr [Gi_rb_bad_map_no_keyinput] = Pr [Gi_rb_bad_map_inline_v].
+Proof.
+  intros.
+Admitted.
+
 (* probability of bad event happening in RB game is bounded by the probability of collisions in a list of length (n+1) of randomly-sampled (Bvector eta) *)
 Lemma Gi_rb_bad_collisions : forall (i : nat),
    Pr  [x <-$ Gi_rb_bad i; ret snd x ] <= Pr_collisions.
@@ -1131,15 +1168,29 @@ Proof.
   rewrite Gi_rb_bad_eq_2.
   rewrite Gi_rb_bad_eq_3.
   rewrite Gi_rb_bad_eq_4.
-  rewrite Gi_rb_bad_eq_5.
+  rewrite Gi_rb_bad_eq_5.       (* questionable *)
   rewrite Gi_rb_bad_eq_6.
-  unfold Gi_rb_bad_map_inline.
-  Opaque hasDups.
-  fcf_inline_first.
-  (* apply Adam's collision bound here *)
+  rewrite Gi_rb_bad_eq_7.
+  rewrite Gi_rb_bad_eq_8.
+  unfold Gi_rb_bad_map_inline_v.
   
-  admit.
-Qed.                            (* for purposes of graphing *)
+  Opaque hasDups.
+  unfold Pr_collisions.
+  Check dupProb.
+  generalize dupProb.
+  intros dupProb.
+
+(* TODO there's a more general lemma *)
+  assert (length (forNats (S blocksPerCall)) = S blocksPerCall).
+  { admit. }
+  rewrite <- H at 2.
+  (* apply Adam's collision bound here *)
+  apply dupProb.
+
+  (* didn't need either of these (work from PRF_DRBG) TODO *)
+  (* apply FixedInRndList_prob. *)
+  (* apply dupProb_const. *)
+Qed.
 
 (* Main theorem (modeled on PRF_DRBG_G3_G4_close) *)
 (* Gi_rf 0:  RF  PRF PRF
@@ -1236,8 +1287,8 @@ Proof.
   unfold Gi_prg.
   comp_skip.
   (* comp_skip. (* ? *) *)
-
-Admitted.
+  admit.
+Qed.
 
 (* ------------------------------- *)
 
